

$$C_e^I \frac{\partial T_e^I}{\partial t} = \frac{\partial}{\partial x} \left(\kappa_e^I \frac{\partial T_e^I}{\partial x} \right) - G^I(T_e^I - T_l^I) + S, \quad (1a)$$

$$C_l^I \frac{\partial T_l^I}{\partial t} = \frac{\partial}{\partial x} \left(\kappa_l^I \frac{\partial T_l^I}{\partial x} \right) + G^I(T_e^I - T_l^I), \quad (1b)$$

$$C_e^{II} \frac{\partial T_e^{II}}{\partial t} = \frac{\partial}{\partial x} \left(\kappa_e^{II} \frac{\partial T_e^{II}}{\partial x} \right) - G^{II}(T_e^{II} - T_l^{II}), \quad (1c)$$

$$C_l^{II} \frac{\partial T_l^{II}}{\partial t} = \frac{\partial}{\partial x} \left(\kappa_l^{II} \frac{\partial T_l^{II}}{\partial x} \right) + G^{II}(T_e^{II} - T_l^{II}). \quad (1d)$$

$$S = \sqrt{\frac{\beta}{\pi}} \frac{(1-R)I_0}{t_p \delta} \exp \left[-\frac{x}{\delta} - \beta \left(\frac{t - 2t_p}{t_p} \right)^2 \right]. \quad (2)$$

$$T_e^I(x, 0) = T_l^I(x, 0) = T_0, \quad (3a)$$

$$T_e^{II}(x, 0) = T_l^{II}(x, 0) = T_0, \quad (3b)$$

$$\frac{\partial T_e^I(x=0, t)}{\partial x} = \frac{\partial T_e^{II}(x=L, t)}{\partial x} = 0, \quad (4a)$$

$$\frac{\partial T_l^I(x=0, t)}{\partial x} = \frac{\partial T_l^{II}(x=L, t)}{\partial x} = 0. \quad (4b)$$

Further, at the interface, i.e., at $x = L_1$, the two layers are in perfect thermal contact, i.e.,

$$T_e^I(x, t) = T_e^{II}(x, t), \quad (5a)$$

$$T_l^I(x, t) = T_l^{II}(x, t), \quad (5b)$$

$$\kappa_e^I \frac{\partial T_e^I(x, t)}{\partial x} = \kappa_e^{II} \frac{\partial T_e^{II}(x, t)}{\partial x}, \quad (5c)$$

$$\kappa_l^I \frac{\partial T_l^I(x, t)}{\partial x} = \kappa_l^{II} \frac{\partial T_l^{II}(x, t)}{\partial x}. \quad (5d)$$